%NOTE
\documentclass{article}
\usepackage[margin=1.0in]{geometry}
\usepackage{titling}
\usepackage{graphicx}
\usepackage{float}
\usepackage[T1]{fontenc}

\begin{document}
	
	%%% title
	\setlength{\droptitle}{-5em}
	\title{R.4 Solving and Factoring}
	\date{}
	\author{}
	\maketitle
	
	%%% first section
		\section*{Quadratic Patterns}
	\textbf{Difference of Squares} \\
	$a^2 - b^2 = (a-b)(a+b)$ \\
	Example: $9x^2 -64 = (3x + 8 )(3x-8)$ \\ \\
	\textbf{Difference of Cubes}\newline
	$a^3 + b^3 = (a+b)(a^2 - ab +b^2)$\\
	(On the right side, first sign is same, second is opposite, last is +). \\
	Example: $2^3 + 5^3 = (2 + 5)(2^2 - 10 + 5^2)$ \\
	\\
	\textbf{Perfect Square Trinomial} \\
	Must satisfy requirement of $b^2=4ac$ \\
	Example: $x^2+6x+9$ \\
	$6^2 = 4*1*9$ $\rightarrow$ $36=36$ \\
	$(x+3)(x+3)$ 
	\section*{Quadratic Methods}
	\textbf{Factor By Grouping} \\
	$3t^3 + 6t^2 + 2t + 4$  \\
	Take out common monomials for first 2 and last 2 (can rearrange nums) \\
	$3t^2(t + 2) + 2(t+2)$ \\
	$(3t^2 + 2) (t+2)$ \\ \\
	\textbf{Into 2 Binomials} \\
	$x^2 + 7x + 12$ \\
	Fill in last number of each paren: $( + 4) ( + 3)$ - have to add to 7, multiply to 12 \\
	$x^2 + bx + c$ \\
	(  +d) (  +e) - D and E have to add up to B and multiply to C \\\\
	\textbf{Quadratic Formula} : $x=\frac{-b\pm\sqrt{b^2-4ac}}{2a}$ \\
	Example: $x^2+3x+2$ \\
	$x=\frac{-3\pm\sqrt{3^2-4*1*2}}{2*1}$ \\
	$x=\frac{-3\pm\sqrt{1}}{2}$ \\
	Finally: $-1$ and $-2$ are returned from the formula. \\ \\
	\textbf{Completing the Square} \\
	Example: $x^2+4x+1$ \\
	1) Divide equation by $a$ \\
	Ex: Skip, $a=1$\\
	2) Move $c$ to the opposite side of the equation \\
	Ex: $x^2+4x = -1$ \\
	3) Create a perfect square trinomial by completing operations on each side \\
	Ex: $x^2 + 4x + 4 = 3$\\
	$(x+2)^2 = \pm 3$\\
	$\rightarrow$ Resulting equation should follow the form $(x + p)^2 = \pm q$\\
	4) $\sqrt{}$ equation \\
	Ex: $x+2 = \pm ~1.73$ \\
	5) Solve for x\\
	Ex: $x = ~-3.73$ or $x = ~-0.27$
	
\end{document}
